tests/programs/58_float_casts.c
@@ -1,0 +1,13 @@
+#include <stdio.h>
+#include <stdint.h>
+int main() {
+    int64_t n = 0, m = 0;
+    double x = 0;
+    n = 42;
+    x = (double)n;
+    m = (int64_t)x;
+    printf("%s = %ld\n", "n", n);
+    printf("%s = %f\n", "x", x);
+    printf("%s = %ld\n", "m", m);
+    return 0;
+}
