tests/programs/61_float_array.c
@@ -1,0 +1,16 @@
+#include <stdio.h>
+#include <stdint.h>
+double A[10];
+int main() {
+    double x = 0, y = 0, z = 0;
+    A[0] = 1.5;
+    A[1] = 2.5;
+    A[2] = 4.0;
+    x = A[0];
+    y = A[1];
+    z = A[2];
+    printf("%s = %f\n", "x", x);
+    printf("%s = %f\n", "y", y);
+    printf("%s = %f\n", "z", z);
+    return 0;
+}
