tests/programs/62_float_array_sum.c
@@ -1,0 +1,21 @@
+#include <stdio.h>
+#include <stdint.h>
+double A[5];
+int main() {
+    double s = 0;
+    int64_t i = 0;
+    A[0] = 1.0;
+    A[1] = 2.0;
+    A[2] = 3.0;
+    A[3] = 4.0;
+    A[4] = 5.0;
+    s = 0.0;
+    i = 0;
+    while (i < 5) {
+        s = s + A[i];
+        i = i + 1;
+    }
+    printf("%s = %f\n", "s", s);
+    printf("%s = %ld\n", "i", i);
+    return 0;
+}
